x

src/circuit.v
@@ -1,17 +1,45 @@
 From research Require Import base.
 
-Inductive ActionResult s t :=
-| Success : s -> t -> ActionResult s t
-| Failure : ActionResult s t.
+(* A result corresponds to whether or not executing an action was aborted or
+   not.
+
+   You may also view a result as a set with either zero or one elements, where
+   Failure corresponds to zero elements and Success coresponds to a singleton
+   set. *)
+Inductive Result s t :=
+| Success : s -> t -> Result s t
+| Failure : Result s t.
+
+Hint Constructors Result : core.
 
 Arguments Success {_ _}.
 Arguments Failure {_ _}.
 
-Definition Action s t := s -> ActionResult s t.
+Local Instance resultElemOf {s t} : ElemOf (s * t) (Result s t) :=
+  fun '(st, v) r =>
+    match r with
+    | Success st' v' => st = st' /\ v = v'
+    | Failure => False
+    end.
 
+Local Instance emptyResult {s t} : Empty (Result s t) := Failure.
+
+(** * The action monad *)
+
+(* We will represent computations in a shallow embedding of Bluespec-style circuits by
+   using state monads equipped with failure (also known as "guarded state monads").
+
+   This will allow us to write imperative style programs for circuits without much hastle.
+
+   The final target language will have sequential semantics as opposed to the serializable
+   semantics between rules in Bluespec.
+ *)
+Definition Action s t := s -> Result s t.
+
+(* Actions form a monad using the following two operators. *)
 Definition ret {s t} (x : t) : Action s t := fun st => Success st x.
 
-Definition bind {s t1 t2} (m : Action s t1) (f : t1 -> Action s t2) :=
+Definition bind {s t1 t2} (m : Action s t1) (f : t1 -> Action s t2) : Action s t2 :=
   fun st =>
     match m st with
     | Success st' v1 => (f v1) st'
@@ -27,24 +55,25 @@ Notation "m >>| f" := (lift f m) (at level 80, only parsing).
 
 Definition pass {s} : Action s unit := ret tt.
 
-Definition abort {s t} : Action s t :=
-  fun st => Failure.
-
-Definition assert {s} (predicate : s -> bool) : Action s unit :=
-  fun st => if predicate st then pass st else abort st.
-
+(* The following are standard operators for state monads. *)
 Definition get {s} : Action s s := fun st => Success st st.
 
 Definition put {s} (st : s) : Action s unit := fun _ => Success st tt.
 
 Definition modify {s} (f : s -> s) : Action s unit := get >>= (fun st => put (f st)).
 
-Definition run {s t} `{Inhabited t} (m : Action s t) (st : s) :=
-  match m st with
-  | Success st' v => (st', v)
-  | Failure => (st, δ)
-  end.
+(* The following operators, [abort], [assert], and [guard], define what it means
+   for an action to fail. *)
+Definition abort {s t} : Action s t :=
+  fun st => Failure.
 
+Definition assert {s} (P : bool) : Action s unit :=
+   if P then pass else abort.
+
+Definition guard {s} (P : s -> bool) : Action s unit :=
+  get >>= (fun st => assert (P st)).
+
+(* [call] allows an action monad to call a different method given a submodule of [s]. *)
 Definition call {s1 s2 t} (proj : s1 -> s2) (meth : Action s2 t)
   `{Setter (R := s1) (T := s2) proj} : Action s1 t :=
   get >>| proj >>=
@@ -54,7 +83,17 @@ Definition call {s1 s2 t} (proj : s1 -> s2) (meth : Action s2 t)
       | Failure => abort
       end.
 
-Arguments call {_ _ _} (_ _) {_} (_).
+Arguments call {_ _ _} (_) {_} (_).
+
+(* Finally, we define what it means to run an action monad to the next state.
+
+   Failure is equivalent to aborting a transaction, so the result is
+   the same state plus some irrelevant value. *)
+Definition run {s t} (m : Action s t) (st : s) :=
+  match m st with
+  | Success st' v => st'
+  | Failure => st
+  end.
 
 Declare Custom Entry bind_expr.
 Declare Custom Entry call_expr.
@@ -69,15 +108,19 @@ Notation "m .( proj )" :=
 Notation "'let%read' x ':=' e1 'in' e2" :=
   (e1 >>= (fun x => e2))
     (at level 80, x pattern, e1 custom bind_expr,
+      e2 at level 200, right associativity,
       only parsing).
 
 Notation "'let%bind' x ':=' e1 'in' e2" :=
   (e1 >>= (fun x => e2))
-    (at level 80, x pattern, only parsing).
+    (at level 80, x pattern,
+      e2 at level 200, right associativity,
+      only parsing).
 
 Notation "'let%map' x ':=' e1 'in' e2" :=
   (e1 >>| (fun x => e2))
-    (at level 80, x pattern, e1 custom bind_expr,
+    (at level 80, x pattern,
+      e2 at level 200, right associativity,
       only parsing).
 
 Notation "'self' ':=' e1" :=
@@ -96,7 +139,7 @@ Notation "'self' .( proj ) '::=' e1" :=
   (modify (set proj e1))
     (at level 200, e1 at level 80, only parsing).
 
-Notation "m1 ';;' m2" := (m1 >>= (fun _ => m2)) (only parsing).
+Notation "m1 ';;' m2" := (m1 >>= (fun _ => m2)) (right associativity, only parsing).
 
 Notation "'self' .( proj ) .( meth )" :=
   (call proj meth)
@@ -109,71 +152,170 @@ Notation "'let%call' x ':=' e1 'in' e2" :=
 
 Notation " 'when' c 'then' e " := (if c then e else pass) (at level 200).
 
-Definition hoare_triple {s t} (P : s -> Prop) (c : Action s t) (Q : t -> s -> Prop) := forall st,
-    P st ->
-    match c st with
-    | Success st' v => Q v st'
-    | Failure => True
-    end.
+(** * Hoare logic over action monads *)
+Definition Assertion {s} := s -> Prop.
 
-Notation "{{ P }} c {{ Q }}" := (hoare_triple P c Q) (at level 90, c at next level).
+(* We can give partial correctness specifications to actions in the form of
+   preconditions and postconditions to the execution of a particular action. *)
+Definition hoareTriple {s t} (P : Assertion) (c : Action s t) (Q : t -> Assertion) :=
+  forall st, P st -> forall st' v, (st', v) ∈ c st -> Q v st'.
 
-Theorem hoare_consequence {s t} : forall P (c : Action s t) Q P' Q',
+Notation "{{ P }} c {{ Q }}" := (hoareTriple P c Q) (at level 90, c at next level).
+
+Theorem hoareConsequence {s t} : forall  (c : Action s t) P Q P' Q',
     {{ P }} c {{ Q }}
     -> (forall st, P' st -> P st)
     -> (forall v st, Q v st -> Q' v st)
     -> {{ P' }} c {{ Q' }}.
 Proof.
-  cbv [ hoare_triple ].
-  intros.
+  cbv [ hoareTriple elem_of ].
+  simplify.
   specialize H with (st := st).
-  case_match; auto.
+  auto.
 Qed.
 
-Corollary hoare_strengthen {s t} : forall P (c : Action s t) Q Q',
+Corollary hoareStrengthen {s t} : forall P (c : Action s t) Q Q',
     {{ P }} c {{ Q }} -> (forall v st, Q v st -> Q' v st) -> {{ P }} c {{ Q' }}.
 Proof.
   simplify.
-  eapply hoare_consequence; eauto.
+  eapply hoareConsequence; eauto.
 Qed.
 
-Record Method {s} a t :=
-  { methodName : string
-  ; methodBody : a -> Action s t
-  }.
+(** * Refinement *)
+Class Refines A B := refines : A -> B -> Prop.
+Infix "⊑" := refines.
 
-Notation " 'method' name ' x = body " :=
-  {| methodName := name; methodBody := (fun x => body) |}
-    (at level 100, x pattern).
+Definition actionSimulates {s1 s2 t1 t2}
+  (R : s1 -> s2 -> Prop) (m1 : Action s1 t1) (m2 : Action s2 t2) :=
+  forall st1 st2 st2', R st1 st2 -> st2' = run m2 st2 ->
+    exists st1', st1' = run m1 st1 /\ R st1' st2'.
+
+Instance actionRefines {s1 t1 s2 t2} : Refines (Action s1 t1) (Action s2 t2) :=
+  fun m1 m2 => exists (R : s1 -> s2 -> Prop), actionSimulates R m1 m2.
+
+(* We can construct "circuit" objects for the purpose of verification properties
+   such as showing refinement and stating theorems. *)
+Definition Method (name : string) {s} arg res := arg -> Action s res.
+
+Arguments Method : clear implicits.
+
+Notation " 'method' name := body " :=
+  (body : @Method name _ _ _)
+    (at level 100, name at level 80).
+
+Definition methodSimulates {name s1 s2 arg1 arg2 res1 res2}
+  (R1 : s1 -> s2 -> Prop) (R2 : arg1 -> arg2 -> Prop)
+  (m1 : Method name s1 arg1 res1) (m2 : Method name s2 arg2 res2) :=
+  forall a1 a2, R2 a1 a2 -> actionSimulates R1 (m1 a1) (m2 a2).
+
+Instance methodRefines {name s1 s2 arg1 arg2 res1 res2} :
+  Refines (Method name s1 arg1 res1) (Method name s2 arg2 res2) :=
+  fun m1 m2 => exists (R1 : s1 -> s2 -> Prop) (R2 : arg1 -> arg2 -> Prop),
+      methodSimulates R1 R2 m1 m2.
 
 Inductive Methods {s} : list string -> Type :=
-| MethodsNil : Methods []
-| MethodsCons : forall a t (m : Method (s := s) a t) {names},
-    Methods names
-    -> Methods (methodName (s := s) (a := a) m :: names).
+| MethodsNil  : Methods []
+| MethodsCons : forall name arg res (m : Method name s arg res) {names},
+    Methods names -> Methods (name :: names).
+
+Hint Constructors Methods : core.
 
 Arguments Methods : clear implicits.
 
+Notation "';' m1 ';' .. ';' mn" :=
+  (MethodsCons m1 (.. (MethodsCons mn MethodsNil) ..)) (at level 101).
+
+Inductive methodsSimulates {s1 s2} (R : s1 -> s2 -> Prop) :
+  forall {names}, Methods s1 names -> Methods s2 names -> Prop :=
+| MsNil : methodsSimulates R MethodsNil MethodsNil
+| MsCons :
+  forall {name arg1 arg2 res1 res2 names}
+    (m1 : Method name s1 arg1 res1) (m2 : Method name s2 arg2 res2)
+    (ms1 : Methods s1 names) (ms2 : Methods s2 names)
+    (R2 : arg1 -> arg2 -> Prop),
+    methodSimulates R R2 m1 m2 ->
+    methodsSimulates R ms1 ms2 ->
+    methodsSimulates R (MethodsCons m1 ms1) (MethodsCons m2 ms2).
+
+Hint Constructors methodsSimulates : core.
+
+Instance methodsRefines {s1 s2 names} : Refines (Methods s1 names) (Methods s2 names) :=
+  fun ms1 ms2 => exists (R : s1 -> s2 -> Prop), methodsSimulates R ms1 ms2.
+
 Record Circuit {names : list string} :=
   { circuitState : Type
+  ; circuitEvent : Type
+  ; circuitTrace : circuitState -> list circuitEvent
   ; circuitConstructor : circuitState
   ; circuitMethods : Methods circuitState names
   }.
 
 Arguments Circuit : clear implicits.
 
-Notation "{{ 'rep' = state 'and' 'constructor' = constr ms }}" :=
+Notation "{{ 'self' := state ';' 'trace' := trace ';' 'constructor' := constr ms }}" :=
   {| circuitState := state;
+    circuitEvent := _;
+    circuitTrace := trace;
     circuitConstructor := constr;
     circuitMethods := ms |}.
 
-Notation "'and' m1 'and' .. 'and' mn" :=
-  (MethodsCons m1 (.. (MethodsCons mn MethodsNil) ..)) (at level 101).
+Record circuitSimulates {names} (c1 c2 : Circuit names)
+  (R : circuitState c1 -> circuitState c2 -> Prop) : Prop :=
+  { crConstructors : R (circuitConstructor c1) (circuitConstructor c2)
+  ; crMethods : methodsSimulates R (circuitMethods c1) (circuitMethods c2)
+  }.
 
-Definition counter :=
-  {{ rep = nat
-     and constructor = 0
-     and method "increment" '() = self ::= S
+Instance circuitRefines {names} : Refines (Circuit names) (Circuit names) :=
+  fun c1 c2 => exists R, circuitSimulates c1 c2 R.
+
+Definition counter1 : Circuit _ :=
+  {{ self           := nat
+   ; trace          := const (@nil unit)
+   ; constructor    := 0
+   ; method "val"   := fun _ : () => get
+   ; method "incr1" := fun _ : () => modify S
+   ; method "incr2" := fun _ : () => modify S
+   ; method "reset" := fun _ : () => put 0
   }}.
 
-Eval vm_compute in counter.(circuitMethods).
+Record Counter := { c1 : nat ; c2 : nat }.
+Definition mkCounter := {| c1 := 0 ; c2 := 0 |}.
+Definition counterVal := let%read c1 := self.(c1) in let%read c2 := self.(c2) in ret (c1 + c2).
+Definition counterIncr1 := self.(c1) ::= S.
+Definition counterIncr2 := self.(c2) ::= S.
+Definition counterRst := self.(c1) := 0 ;; self.(c2) := 0.
+
+Definition counter2 : Circuit _ :=
+  {{ self           := Counter
+   ; trace          := const (@nil unit)
+   ; constructor    := mkCounter
+   ; method "val"   := fun _ : () => counterVal
+   ; method "incr1" := fun _ : () => counterIncr1
+   ; method "incr2" := fun _ : () => counterIncr2
+   ; method "reset" := fun _ : () => counterRst
+  }}.
+
+Ltac choose_relation R :=
+  match goal with
+  | [ |- ?a ⊑ ?b ] => exists R
+  | [ |- methodsSimulates _ _ _ ] =>
+      eapply MsCons with (R2 := R);
+      cbv [ methodSimulates actionSimulates ];
+      [ eexists | .. ]
+  end; simplify.
+
+Lemma counterRefines : counter2 ⊑ counter1.
+Proof.
+  choose_relation (fun st1 st2 => st1.(c1) + st1.(c2) = st2).
+  split.
+  equality.
+  choose_relation (fun '() '() => True).
+  equality.
+  choose_relation (fun '() '() => True).
+  equality.
+  choose_relation (fun '() '() => True).
+  propositional.
+  choose_relation (fun '() '() => True).
+  equality.
+  constructor.
+Qed.
